Clean up Types

src/Types.v
@@ -1,5 +1,6 @@
 (** * Types as closures *)
 
+Require Import Coq.Classes.Morphisms.
 Require Export Constructor.
 Open Scope code_scope.
 
@@ -9,59 +10,143 @@ Definition closure {Var : Set} (a : Code Var) := I [= a /\ a o a == a.
 Definition fixes {Var : Set} (a : Code Var) (x : Code Var) := a*x == x.
 Notation "x :: a" := (fixes a x) : code_scope.
 
+Instance closure_proper_eq (Var : Set) :
+  Proper (code_eq ==> iff) (@closure Var).
+Proof.
+  simpl_relation; unfold closure; split; intros [Hn Hi]; split;
+  (rewrite -> H || rewrite <- H); auto.
+Qed.
+
+Instance fixes_proper_eq (Var : Set) :
+  Proper (code_eq ==> code_eq ==> iff) (@fixes Var).
+Proof.
+  unfold fixes; intros a a' Ha x x' Hx.
+  rewrite Ha; rewrite Hx; firstorder.
+Qed.
+
 (** ** Atomic types *)
+
+(** [I] is the largest type. *)
+
+Lemma I_nondecreasing (Var : Set) : I [= (I : Code Var).
+Proof. auto. Qed.
+
+Lemma I_idempotent (Var : Set) : I o I == (I : Code Var).
+Proof. beta_eta. Qed.
+Hint Rewrite I_nondecreasing.
 
 Lemma I_closure {Var : Set} : closure (I : Code Var).
 Proof.
-  unfold closure; split.
-  apply code_le_refl.
-  eta_expand; beta_reduce; auto.
+  split; [apply I_nondecreasing | apply I_idempotent].
 Qed.
 
 Theorem I_inhab (Var : Set) (x : Code Var) : x :: I <-> True.
 Proof.
-  unfold fixes.
-  beta_reduce; firstorder.
+  unfold fixes; beta_reduce; firstorder.
 Qed.
 
-Lemma V_closure (Var : Set) : closure (V : Code Var).
+(** [V] is the type of all types *)
+
+Lemma V_nondecreasing (Var : Set) : I [= (V : Code Var).
 Proof.
-  unfold closure.
-  split.
-  (* TODO adapt Y_fix, eta, beta tactics from Points to Codes.
-    unfold V; rewrite Y_fix; rewrite Y_fix; fold V.
-    freeze V in (compute; eta_expand as f; eta_expand as x; beta_reduce).
-    apply LESS_trans with (x || f * x); monotonicity; auto.
-  TODO
-  *)
+  eta_expand as a.
+  rewrite beta_v; rewrite pi_j_right.
+  rewrite beta_v; rewrite pi_j_left.
+  beta_eta.
+Qed.
+
+Lemma V_idempotent (Var : Set) : V o V == (V : Code Var).
+Proof.
+  eta_expand as a; rewrite beta_b.
+Admitted.
+Hint Rewrite V_nondecreasing.
+
+Lemma V_closure {Var : Set} : closure (V : Code Var).
+Proof.
+  split; [apply V_nondecreasing | apply V_idempotent].
+Qed.
+
+Lemma V_sound (Var : Set) (x : Code Var) : x :: V -> closure x.
+Proof.
+  unfold fixes, closure.
+  intros Hfix.
+  assert (I [= x).
+    rewrite <- Hfix; rewrite beta_v; auto.
+  split; auto.
+  rewrite <- Hfix at 3; rewrite beta_v; rewrite Hfix.
+  split; auto.
+  apply code_le_j_ub; auto.
+  rewrite <- I_idempotent.
+  monotonicity; auto.
+Qed.
+
+Lemma V_complete (Var : Set) (x : Code Var) : closure x -> x :: V.
+Proof.
+  unfold fixes, closure; intros [Hn Hi].
 Admitted.
 
 Theorem V_inhab (Var : Set) (x : Code Var) : x :: V <-> closure x.
 Proof.
-  unfold fixes; unfold closure.
-  split.
-    intros Hfix; rewrite <- Hfix; clear Hfix.
-    split.
-  (* TODO *)
-Admitted.
+  split; [apply V_sound | apply V_complete].
+Qed.
 
 Corollary fixes_V_V (Var : Set) : fixes V (V : Code Var).
 Proof.
-  apply V_inhab.
-  apply V_closure.
+  apply V_inhab; apply V_closure.
 Qed.
 
+(** [semi] is Sierpinsky space, inhabited by [{BOT, I, TOP}]. *)
+
 Section semi.
-  Variable Var : Set.
+  Context {Var : Set}.
   Let a := make_var Var 0.
   Let a' := make_var Var 1.
-  Definition Semi := close (\\a,a'; a --> a').
+  Definition semi := Eval compute in close (\\a,a'; a --> a').
 End semi.
-Definition semi {Var : Set} := Semi Var.
 
-Lemma semi_closure (Var : Set) : closure (semi : Code Var).
+Lemma semi_nondecreasing (Var : Set) : I [= (semi : Code Var).
 Proof.
-  (* TODO *)
+  unfold semi.
+  eta_expand as a.
+  rewrite beta_y; rewrite pi_j_left.
+  rewrite beta_j_ap.
+  repeat rewrite pi_j_left.
+  beta_simpl.
+  beta_eta.
+Qed.
+
+Lemma semi_idempotent (Var : Set) : semi o semi == (semi : Code Var).
+Proof.
+  eta_expand as a; rewrite beta_b.
+Admitted.
+Hint Rewrite semi_nondecreasing.
+
+Lemma semi_closure {Var : Set} : closure (semi : Code Var).
+Proof.
+  split; [apply semi_nondecreasing | apply semi_idempotent].
+Qed.
+
+Lemma semi_inhab_bot (Var : Set) : BOT :: (semi : Code Var).
+Proof.
+  unfold semi.
+Admitted.
+
+Lemma semi_inhab_i (Var : Set) : I :: (semi : Code Var).
+Proof.
+  unfold semi.
+Admitted.
+
+Lemma semi_inhab_top (Var : Set) : TOP :: (semi : Code Var).
+Proof.
+  unfold semi.
+Admitted.
+
+Theorem semi_sound (Var : Set) (x : Code Var) : x :: semi ->
+  x == BOT \/
+  x == I \/
+  x == TOP.
+Proof.
+  intros H; unfold fixes in H.
 Admitted.
 
 Theorem semi_inhab (Var : Set) (x : Code Var) : x :: semi <->
@@ -70,20 +155,79 @@ Theorem semi_inhab (Var : Set) (x : Code Var) : x :: semi <->
   x == TOP.
 Proof.
   split.
-  (* TODO *)
-Admitted.
+    apply semi_sound.
+  intro H; destruct H as [Hb | [Hi | Ht]].
+  rewrite Hb; apply semi_inhab_bot.
+  rewrite Hi; apply semi_inhab_i.
+  rewrite Ht; apply semi_inhab_top.
+Qed.
+
+(** [boool] is the set of ambiguous boolean values [K], [F], and [J].
+    We will later define a stricter [bool] that raises [J] to [TOP],
+    i.e., raising an error on ambiguous values. *)
 
 Section boool.
-  Variable Var : Set.
+  Context {Var : Set}.
   Let a := make_var Var 0.
   Let a' := make_var Var 1.
-  Definition Boool := close (\\a,a'; a --> a --> a').
+  Definition boool := Eval compute in close (\\a,a'; a --> a --> a').
 End boool.
-Definition boool {Var : Set} := Boool Var.
 
-Lemma boool_closure (Var : Set) : closure (boool : Code Var).
+Lemma boool_nondecreasing (Var : Set) : I [= (boool : Code Var).
 Proof.
-  (* TODO *)
+  unfold boool.
+  eta_expand as a.
+  rewrite beta_y; rewrite pi_j_left.
+  rewrite beta_j_ap.
+  repeat rewrite pi_j_left.
+  beta_simpl.
+  beta_eta.
+Qed.
+
+Lemma boool_idempotent (Var : Set) : boool o boool == (boool : Code Var).
+Proof.
+  eta_expand as a; rewrite beta_b.
+Admitted.
+Hint Rewrite boool_nondecreasing.
+
+Lemma boool_closure {Var : Set} : closure (boool : Code Var).
+Proof.
+  split; [apply boool_nondecreasing | apply boool_idempotent].
+Qed.
+
+Lemma boool_inhab_bot (Var : Set) : BOT :: (boool : Code Var).
+Proof.
+  unfold boool.
+Admitted.
+
+Lemma boool_inhab_k (Var : Set) : K :: (boool : Code Var).
+Proof.
+  unfold boool.
+Admitted.
+
+Lemma boool_inhab_f (Var : Set) : K * I :: (boool : Code Var).
+Proof.
+  unfold boool.
+Admitted.
+
+Lemma boool_inhab_j (Var : Set) : J :: (boool : Code Var).
+Proof.
+  unfold boool.
+Admitted.
+
+Lemma boool_inhab_top (Var : Set) : TOP :: (boool : Code Var).
+Proof.
+  unfold boool.
+Admitted.
+
+Theorem boool_sound (Var : Set) (x : Code Var) : x :: boool ->
+  x == BOT \/
+  x == K \/
+  x == K * I \/
+  x == J \/
+  x == TOP.
+Proof.
+  intros H; unfold fixes in H.
 Admitted.
 
 Theorem boool_inhab (Var : Set) (x : Code Var) : x :: boool <->
@@ -94,5 +238,11 @@ Theorem boool_inhab (Var : Set) (x : Code Var) : x :: boool <->
   x == TOP.
 Proof.
   split.
-  (* TODO *)
-Admitted.
+    apply boool_sound.
+  intro H; destruct H as [Hb |[ Hk |[ Hf |[ Hj | Ht]]]].
+  rewrite Hb; apply boool_inhab_bot.
+  rewrite Hk; apply boool_inhab_k.
+  rewrite Hf; apply boool_inhab_f.
+  rewrite Hj; apply boool_inhab_j.
+  rewrite Ht; apply boool_inhab_top.
+Qed.
